details towards functional testing

src/tls/Negotiation.fst
@@ -2365,7 +2365,7 @@ let server_hrr_verify offer mode hrr =
 
 //19-06-17 Verification of this function is particularly slow and brittle; what to do? 
 #reset-options "--z3rlimit 300"
-let server_ClientHello #region ns offer log =
+let server_ClientHello #region ns offer log0 =
   trace ("offered client extensions "^string_of_ches offer.CH.extensions);
   trace ("offered cipher suites "^string_of_ciphersuitenames offer.CH.cipher_suites);
   trace (match find_supported_groups offer with
@@ -2385,9 +2385,11 @@ let server_ClientHello #region ns offer log =
     | Error z -> trace ("negotiation failed: "^string_of_error z); Error z
     | Correct r -> (
       let h = get() in assert (inv ns h);
+      // TRANSCRIPT:
+      // let tr = Transcript.create (ha_of_sm sm) in // { state(tr) == Start(None) }
       let stateless_retry = 
         match find_cookie offer with
-        | None -> None
+        | None -> None 
         | Some c ->
           // stateless HRR.
           match TLS.Cookie.decrypt c with
@@ -2399,21 +2401,31 @@ let server_ClientHello #region ns offer log =
           | Correct (digest, extra, hrr) ->
             trace ("Loaded stateless retry cookie "^hex_of_bytes extra);
             trace ("Setting transcript to CH1 hash "^hex_of_bytes digest);
+            // TODO check consistency of sm with hrr's cs and group;
+            // this is required to enforce the earlier server policy.
 
-            // TODO check consistency of sm with hrr's cs and group; this is required to enforce 
-            // the earlier server policy. 
+            // Lowering: we can use the output buffer as scratch space
+            // for outputting the digest (of known size) and the hrr
+            // (possibly quite large), since we only need them for
+            // computing the transcript digest.
+            //
+            // Alternatively, we could pass the hrr in two chunks: the
+            // (small, reconstructed) hrr prefix, and the (received)
+            // encrypted cookie.
+            //
+            // TRANSCRIPT 
+            // extend_stateless hrr digest hrr //{ Start(None) --HRR digest hrr--> Start(Some(digest,hrr)) }
+            // using sm's hash algorithm. 
+
+            //FIXME! can't prove [writing] without a precondition. The whole function TCs without these 3 lines.
+            let h0 = get() in assume HandshakeLog.(writing h0 log0 /\ valid_transcript (transcript h0 log0)); 
+            HandshakeLog.load_stateless_cookie log0 hrr digest;
+            assume False; 
+            Some extra // to be passed to the server nego callback
             
-            // TODO create Transcript in state Start(Some(digest,hrr))
-            // using sm's hash algorithm. Lower: consider taking the
-            // (decrypted) digest, (small, reconstructed) hrr prefix,
-            // and (received) encrypted cookie from three different
-            // const_buffers.
-
-            //FIXME! can't prove [writing] without a precondition
-            // HandshakeLog.load_stateless_cookie log hrr digest;
-            // we will pass extra to the server nego callback
-            Some extra 
         in 
+      // TRANSCRIPT 
+      // extend_ch offer //{ Start(r) --> ClientHello(r,offer) }
       let h = get() in assert (inv ns h);
       match r with 
       | ServerRetry hrr -> (
@@ -2426,7 +2438,7 @@ let server_ClientHello #region ns offer log =
           trace ("no common group, sending a retry request...");
           // TODO create Transcript in state Start(Some(digest,hrr)) to compute this digest
           let ha = TLS.Cookie.hrr_ha hrr in 
-          let digest = HandshakeLog.hash_tag #ha log in 
+          let digest = HandshakeLog.hash_tag #ha log0 in 
           let hrr = TLS.Cookie.append digest empty_bytes hrr in
           ns.state := S_HRR offer hrr;
           sm ))
@@ -2451,7 +2463,7 @@ let server_ClientHello #region ns offer log =
           assume(CipherSuite13? m.n_cipher_suite); // from ServerMode 
           let hrr = TLS.Cookie.hrr0 offer.CH.session_id m.n_cipher_suite in
           let ha = TLS.Cookie.hrr_ha hrr in 
-          let digest = HandshakeLog.hash_tag #ha log in
+          let digest = HandshakeLog.hash_tag #ha log0 in
           let hrr = TLS.Cookie.append digest filling hrr in
           ns.state := S_HRR offer hrr;
           Correct (ServerRetry hrr))
